Update about rsc.

SfLib.v
@@ -247,3 +247,56 @@ Proof.
       apply (IHn' m').
       apply H. apply LE.
 Qed.
+
+Inductive appears_in (n : nat) : list nat -> Prop :=
+| ai_here : forall l, appears_in n (n::l)
+| ai_later : forall m l, appears_in n l -> appears_in n (m::l).
+
+Definition relation (X:Type) := X -> X -> Prop.
+
+Definition partial_function {X: Type} (R: relation X) :=
+  forall x y1 y2 : X, R x y1 -> R x y2 -> y1 = y2.
+
+Inductive next_nat (n:nat) : nat -> Prop :=
+| nn : next_nat n (S n).
+
+Inductive total_relation : nat -> nat -> Prop :=
+  tot : forall n m : nat, total_relation n m.
+
+Inductive empty_relation : nat -> nat -> Prop := .
+
+Inductive refl_step_closure (X:Type) (R: relation X)
+                            : X -> X -> Prop :=
+  | rsc_refl : forall (x : X),
+                 refl_step_closure X R x x
+  | rsc_step : forall (x y z : X),
+                    R x y ->
+                    refl_step_closure X R y z ->
+                    refl_step_closure X R x z.
+Implicit Arguments refl_step_closure [[X]].
+
+Tactic Notation "rsc_cases" tactic(first) ident(c) :=
+  first;
+  [ Case_aux c "rsc_refl" | Case_aux c "rsc_step" ].
+
+Theorem rsc_R : forall (X:Type) (R:relation X) (x y : X),
+       R x y -> refl_step_closure R x y.
+Proof.
+  intros X R x y r.
+  apply rsc_step with y. apply r. apply rsc_refl. Qed.
+
+Theorem rsc_trans :
+  forall (X:Type) (R: relation X) (x y z : X),
+      refl_step_closure R x y ->
+      refl_step_closure R y z ->
+      refl_step_closure R x z.
+Proof.
+  intros X R x y z cx.
+  generalize dependent z.
+  induction cx as [x0| s t u rST cTU].
+  (* refl *) intros z H. apply H.
+  (* step *)
+    intros z cUZ.
+    apply rsc_step with (y:=t).
+    apply rST. apply IHcTU. apply cUZ.
+Qed.
